proof of unitary to nd semantics

NDSem.v
@@ -8,28 +8,60 @@ Require Import UnitarySem.
 Definition norm {n} (ψ : Vector n) :=
   sqrt (fst (ψ ∘ ψ†)).  
 
+Open Scope com.
+
 (* With scaling *)
+
 Reserved Notation "c '/' ψ '⇩' ψ'"
                   (at level 40, ψ at level 39).
 
 Inductive nd_eval {dim : nat} : com -> Vector (2^dim) -> Vector (2^dim) -> Prop :=
   | nd_skip : forall ψ, nd_eval skip ψ ψ
   | nd_app : forall n (u : Unitary n) (l : list nat) (ψ : Vector (2^dim)),
-      (app u l) / ψ ⇩ ((ueval dim u l) × ψ)
+      app u l / ψ ⇩ ((ueval dim u l) × ψ)
   | nd_meas0 : forall n (ψ : Vector (2^dim)),
       let ψ' := @pad 2 n dim (∣0⟩⟨0∣) × ψ in 
       norm ψ' <> 0%R ->
-      (meas n) / ψ ⇩ (scale (/(norm ψ')) ψ') 
+      meas n / ψ ⇩ (scale (/(norm ψ')) ψ') 
   | nd_meas1 : forall n (ψ : Vector (2^dim)),
       let ψ' := @pad 2 n dim (∣1⟩⟨1∣) × ψ in
       norm ψ' <> 0%R ->
-      (meas n) / ψ ⇩ (scale (/(norm ψ')) ψ') 
+      meas n / ψ ⇩ (scale (/(norm ψ')) ψ') 
   | nd_reset0 : forall n (ψ : Vector (2^dim)),
       let ψ' := @pad 2 n dim (∣0⟩⟨0∣) × ψ in 
-      (meas n) / ψ ⇩ (scale (/(norm ψ')) ψ') 
+      meas n / ψ ⇩ (scale (/(norm ψ')) ψ') 
   | nd_reset1 : forall n (ψ : Vector (2^dim)),
       let ψ' := @pad 2 n dim (∣0⟩⟨1∣) × ψ in (* is this right? *)
       norm ψ' <> 0%R ->
-      (meas n) / ψ ⇩ (scale (/(norm ψ')) ψ')
+      meas n / ψ ⇩ (scale (/(norm ψ')) ψ')
+  | nd_seq : forall (c1 c2 : com) (ψ ψ' ψ'' : Vector (2^dim)),
+      c1 / ψ ⇩ ψ' ->
+      c2 / ψ' ⇩ ψ'' ->
+      (c1 ; c2) / ψ ⇩ ψ''
 
 where "c '/' ψ '⇩' ψ'" := (nd_eval c ψ ψ').              
+
+Lemma nd_eval_ucom : forall (c : ucom) (dim : nat) (ψ ψ' : Vector (2^dim)),
+    WF_Matrix _ _ ψ ->
+    c / ψ ⇩ ψ' <-> (uc_eval dim c) × ψ = ψ'.
+Proof.
+  intros c dim ψ ψ' WF.
+  split; intros H.
+  - gen ψ' ψ.
+    induction c; intros ψ' ψ WF E; dependent destruction E; subst.
+    + simpl; Msimpl; easy.
+    + simpl.
+      rewrite Mmult_assoc.
+      rewrite (IHc1 ψ'); trivial. 
+      assert (WF_Matrix _ _ ψ') by (rewrite <- (IHc1 _ ψ) ; auto with wf_db).      
+      rewrite (IHc2 ψ''); easy.
+    + easy.
+  - gen ψ' ψ.
+    induction c; intros ψ' ψ WF E; subst.
+    + simpl; Msimpl. constructor.
+    + apply nd_seq with (uc_eval dim c1 × ψ).
+      apply IHc1; trivial.
+      apply IHc2; auto with wf_db.
+      simpl; rewrite Mmult_assoc; easy.
+    + simpl; constructor.
+Qed.
